books/projects/x86isa/machine/instructions/bit.lisp
@@ -321,348 +321,406 @@
        (x86 (write-*ip proc-mode temp-rip x86)))
     x86))
 
-(skip-proofs
-  (def-inst x86-bt-0F-B3
+;; Used to prove some guards in the following
+(local (defthm integerp-ash
+               (integerp (ash x c))))
 
-            ;; 0F B3/r: BTR r/m16, r16
-            ;; 0F B3/r: BTR r/m32, r32
-            ;; REX.W + 0F B3/r: BTR r/m64, r64
+(def-inst x86-bt-0F-B3
 
-            :parents (two-byte-opcodes)
+          ;; 0F B3/r: BTR r/m16, r16
+          ;; 0F B3/r: BTR r/m32, r32
+          ;; REX.W + 0F B3/r: BTR r/m64, r64
 
-            :returns (x86 x86p :hyp (x86p x86))
+          :parents (two-byte-opcodes)
 
-            :guard-hints (("Goal" :in-theory (enable rme-size-of-1-to-rme08)))
+          :returns (x86 x86p :hyp (x86p x86))
 
-            :modr/m t
+          :guard-hints (("Goal" :in-theory (enable rme-size-of-1-to-rme08)))
 
-            :body
+          :modr/m t
 
-            (b* (((the (integer 1 8) operand-size)
-                  (select-operand-size
-                    proc-mode nil rex-byte nil prefixes nil nil nil x86))
+          :body
 
-                 (p2 (prefixes->seg prefixes))
-                 (p4? (equal #.*addr-size-override*
-                             (prefixes->adr prefixes)))
+          (b* (((the (integer 1 8) operand-size)
+                (select-operand-size
+                  proc-mode nil rex-byte nil prefixes nil nil nil x86))
 
-                 (seg-reg (select-segment-register proc-mode p2 p4? mod r/m sib x86))
+               (p2 (prefixes->seg prefixes))
+               (p4? (equal #.*addr-size-override*
+                           (prefixes->adr prefixes)))
 
-                 (inst-ac? t)
-                 ((mv flg0
-                      bitBase
-                      (the (unsigned-byte 3) increment-RIP-by)
-                      (the (signed-byte 64) addr)
-                      x86)
-                  (x86-operand-from-modr/m-and-sib-bytes
-                    proc-mode #.*gpr-access* operand-size inst-ac?
-                    nil ;; Not a memory pointer operand
-                    seg-reg p4? temp-rip rex-byte r/m mod sib
-                    0 ;; No immediate data
-                    x86))
-                 ((when flg0)
-                  (!!ms-fresh :x86-operand-from-modr/m-and-sib-bytes flg0))
+               (seg-reg (select-segment-register proc-mode p2 p4? mod r/m sib x86))
 
-                 (bitOffset (rgfi-size operand-size (reg-index reg rex-byte *r*) rex-byte x86))
+               (inst-ac? t)
+               ((mv flg0
+                    bitBase
+                    (the (unsigned-byte 3) increment-RIP-by)
+                    (the (signed-byte 64) addr)
+                    x86)
+                (x86-operand-from-modr/m-and-sib-bytes
+                  proc-mode #.*gpr-access* operand-size inst-ac?
+                  nil ;; Not a memory pointer operand
+                  seg-reg p4? temp-rip rex-byte r/m mod sib
+                  0 ;; No immediate data
+                  x86))
+               ((when flg0)
+                (!!ms-fresh :x86-operand-from-modr/m-and-sib-bytes flg0))
 
-                 ((mv flg (the (signed-byte #.*max-linear-address-size*) temp-rip))
-                  (add-to-*ip proc-mode temp-rip increment-RIP-by x86))
-                 ((when flg) (!!ms-fresh :rip-increment-error temp-rip))
+               (bitOffset (rgfi-size operand-size (reg-index reg rex-byte *r*) rex-byte x86))
 
-                 (badlength? (check-instruction-length start-rip temp-rip 0))
-                 ((when badlength?)
-                  (!!fault-fresh :gp 0 :instruction-length badlength?)) ;; #GP(0)
+               ((mv flg (the (signed-byte #.*max-linear-address-size*) temp-rip))
+                (add-to-*ip proc-mode temp-rip increment-RIP-by x86))
+               ((when flg) (!!ms-fresh :rip-increment-error temp-rip))
 
-                 ((the (integer 0 64) bitOffset)
-                  (mod bitOffset (the (integer 0 64) (ash operand-size 3))))
+               (badlength? (check-instruction-length start-rip temp-rip 0))
+               ((when badlength?)
+                (!!fault-fresh :gp 0 :instruction-length badlength?)) ;; #GP(0)
 
-                 ;; Update the x86 state:
-                 ;; CF affected. ZF unchanged. PF, AF, SF, and OF undefined.
-                 ;; If reg is 5, we need to set the selected bit
-                 ;; If reg is 6, we need to clear the selected bit
-                 (x86
-                   (let* ((x86 (!flgi :cf
-                                      (the (unsigned-byte 1)
-                                           (acl2::logbit bitOffset bitBase))
-                                      x86))
-                          (x86 (!flgi-undefined :pf x86))
-                          (x86 (!flgi-undefined :af x86))
-                          (x86 (!flgi-undefined :sf x86))
-                          (x86 (!flgi-undefined :of x86)))
-                     x86))
-                 ((mv flg x86) (x86-operand-to-reg/mem
+               ((the (integer 0 64) bitOffset)
+                (mod bitOffset (the (integer 0 64) (ash operand-size 3))))
+
+               ;; Update the x86 state:
+               ;; CF affected. ZF unchanged. PF, AF, SF, and OF undefined.
+               ;; If reg is 5, we need to set the selected bit
+               ;; If reg is 6, we need to clear the selected bit
+               (x86
+                 (let* ((x86 (!flgi :cf
+                                    (the (unsigned-byte 1)
+                                         (acl2::logbit bitOffset bitBase))
+                                    x86))
+                        (x86 (!flgi-undefined :pf x86))
+                        (x86 (!flgi-undefined :af x86))
+                        (x86 (!flgi-undefined :sf x86))
+                        (x86 (!flgi-undefined :of x86)))
+                   x86))
+               ((mv flg x86) (x86-operand-to-reg/mem
+                               proc-mode
+                               operand-size
+                               inst-ac?
+                               nil
+                               (logand bitBase
+                                       (lognot (ash 1 bitOffset)))
+                               seg-reg
+                               addr
+                               rex-byte
+                               r/m
+                               mod
+                               x86))
+               ((when flg) (!!ms-fresh :x86-operand-to-reg/mem flg))
+               (x86 (write-*ip proc-mode temp-rip x86)))
+              x86))
+
+(def-inst x86-bt-0F-BA
+
+          ;; 0F BA/4: BT r/m16/32/64, imm8
+          ;; 0F BA/5: BTS r/m16/32/64, imm8
+          ;; 0F BA/6: BTR r/m16/32/64, imm8
+
+          ;; If the bitBase is a register, the BitOffset can be in the range 0
+          ;; to [15, 31, 63] depending on the mode and register size.  If the
+          ;; bitBase is a memory address and bitOffset is an immediate operand,
+          ;; then also the bitOffset can be in the range 0 to [15, 31, 63].
+
+          :parents (two-byte-opcodes)
+
+          :returns (x86 x86p :hyp (x86p x86))
+
+          :guard-hints (("Goal" :in-theory (e/d* () (signed-byte-p unsigned-byte-p))))
+
+          :prepwork
+          ((local (defthm unsigned-byte-p-logior-unsigned-byteps
+                          (implies (and (natp i)
+                                        (unsigned-byte-p i x)
+                                        (unsigned-byte-p i y))
+                                   (unsigned-byte-p i (logior x y)))))
+
+          :modr/m t
+
+          :body
+
+          ;; Note: opcode is the second byte of the two-byte opcode.
+
+          (b* (((the (integer 1 8) operand-size)
+                (select-operand-size
+                  proc-mode nil rex-byte nil prefixes nil nil nil x86))
+
+               (log2-operand-size (case operand-size
+                                    (1 0)
+                                    (2 1)
+                                    (4 2)
+                                    (8 3)))
+
+               (p2 (prefixes->seg prefixes))
+               (p4? (equal #.*addr-size-override*
+                           (prefixes->adr prefixes)))
+
+               (seg-reg (select-segment-register proc-mode p2 p4? mod r/m sib x86))
+
+               (inst-ac? t)
+               ((mv flg0
+                    bitBase
+                    (the (unsigned-byte 3) increment-RIP-by)
+                    (the (signed-byte 64) addr)
+                    x86)
+                (x86-operand-from-modr/m-and-sib-bytes
+                  proc-mode #.*gpr-access* operand-size inst-ac?
+                  nil ;; Not a memory pointer operand
+                  seg-reg p4? temp-rip rex-byte r/m mod sib
+                  1 ;; One-byte immediate data
+                  x86))
+               ((when flg0)
+                (!!ms-fresh :x86-operand-from-modr/m-and-sib-bytes flg0))
+
+               ((mv flg (the (signed-byte #.*max-linear-address-size*) temp-rip))
+                (add-to-*ip proc-mode temp-rip increment-RIP-by x86))
+               ((when flg) (!!ms-fresh :rip-increment-error temp-rip))
+
+               ((mv flg1 (the (unsigned-byte 8) bitOffset) x86)
+                (rme-size-opt proc-mode 1 temp-rip #.*cs* :x nil x86))
+               ((when flg1) (!!ms-fresh :rme-size-error flg1))
+
+               ((mv flg (the (signed-byte #.*max-linear-address-size*) temp-rip))
+                (add-to-*ip proc-mode temp-rip 1 x86))
+               ((when flg) (!!ms-fresh :rip-increment-error temp-rip))
+
+               (badlength? (check-instruction-length start-rip temp-rip 0))
+               ((when badlength?)
+                (!!fault-fresh :gp 0 :instruction-length badlength?)) ;; #GP(0)
+
+               ((the (integer 0 64) bitOffset)
+                (loghead (+ log2-operand-size 3)
+                         bitOffset))
+
+               ;; Update the x86 state:
+               ;; CF affected. ZF unchanged. PF, AF, SF, and OF undefined.
+               ;; If reg is 5, we need to set the selected bit
+               ;; If reg is 6, we need to clear the selected bit
+               (x86
+                 (let* ((x86 (!flgi :cf
+                                    (the (unsigned-byte 1)
+                                         (acl2::logbit bitOffset bitBase))
+                                    x86))
+                        (x86 (!flgi-undefined :pf x86))
+                        (x86 (!flgi-undefined :af x86))
+                        (x86 (!flgi-undefined :sf x86))
+                        (x86 (!flgi-undefined :of x86)))
+                   x86))
+               ((mv flg x86) (if (member reg '(5 6))  ;; If BTR, we need to clear the tested bit
+                               (x86-operand-to-reg/mem
                                  proc-mode
                                  operand-size
                                  inst-ac?
                                  nil
-                                 (logand bitBase
-                                         (lognot (ash 1 bitOffset)))
+                                 (if (equal reg 5)
+                                   (logior bitBase
+                                           (ash 1 bitOffset))
+                                   (logand bitBase
+                                           (lognot (ash 1 bitOffset))))
                                  seg-reg
                                  addr
                                  rex-byte
                                  r/m
                                  mod
-                                 x86))
-                 ((when flg) (!!ms-fresh :x86-operand-to-reg/mem flg))
-                 (x86 (write-*ip proc-mode temp-rip x86)))
-                x86)))
-(skip-proofs
-  (def-inst x86-bt-0F-BA
-
-            ;; 0F BA/4: BT r/m16/32/64, imm8
-            ;; 0F BA/5: BTS r/m16/32/64, imm8
-            ;; 0F BA/6: BTR r/m16/32/64, imm8
-
-            ;; If the bitBase is a register, the BitOffset can be in the range 0
-            ;; to [15, 31, 63] depending on the mode and register size.  If the
-            ;; bitBase is a memory address and bitOffset is an immediate operand,
-            ;; then also the bitOffset can be in the range 0 to [15, 31, 63].
-
-            :parents (two-byte-opcodes)
-
-            :returns (x86 x86p :hyp (x86p x86))
-
-            :guard-hints (("Goal" :in-theory (enable rme-size-of-1-to-rme08)))
-
-            :modr/m t
-
-            :body
-
-            ;; Note: opcode is the second byte of the two-byte opcode.
-
-            (b* (((the (integer 1 8) operand-size)
-                  (select-operand-size
-                    proc-mode nil rex-byte nil prefixes nil nil nil x86))
-
-                 (p2 (prefixes->seg prefixes))
-                 (p4? (equal #.*addr-size-override*
-                             (prefixes->adr prefixes)))
-
-                 (seg-reg (select-segment-register proc-mode p2 p4? mod r/m sib x86))
-
-                 (inst-ac? t)
-                 ((mv flg0
-                      bitBase
-                      (the (unsigned-byte 3) increment-RIP-by)
-                      (the (signed-byte 64) addr)
-                      x86)
-                  (x86-operand-from-modr/m-and-sib-bytes
-                    proc-mode #.*gpr-access* operand-size inst-ac?
-                    nil ;; Not a memory pointer operand
-                    seg-reg p4? temp-rip rex-byte r/m mod sib
-                    1 ;; One-byte immediate data
-                    x86))
-                 ((when flg0)
-                  (!!ms-fresh :x86-operand-from-modr/m-and-sib-bytes flg0))
-
-                 ((mv flg (the (signed-byte #.*max-linear-address-size*) temp-rip))
-                  (add-to-*ip proc-mode temp-rip increment-RIP-by x86))
-                 ((when flg) (!!ms-fresh :rip-increment-error temp-rip))
-
-                 ((mv flg1 (the (unsigned-byte 8) bitOffset) x86)
-                  (rme-size-opt proc-mode 1 temp-rip #.*cs* :x nil x86))
-                 ((when flg1) (!!ms-fresh :rme-size-error flg1))
-
-                 ((mv flg (the (signed-byte #.*max-linear-address-size*) temp-rip))
-                  (add-to-*ip proc-mode temp-rip 1 x86))
-                 ((when flg) (!!ms-fresh :rip-increment-error temp-rip))
-
-                 (badlength? (check-instruction-length start-rip temp-rip 0))
-                 ((when badlength?)
-                  (!!fault-fresh :gp 0 :instruction-length badlength?)) ;; #GP(0)
-
-                 ((the (integer 0 64) bitOffset)
-                  (mod bitOffset (the (integer 0 64) (ash operand-size 3))))
-
-                 ;; Update the x86 state:
-                 ;; CF affected. ZF unchanged. PF, AF, SF, and OF undefined.
-                 ;; If reg is 5, we need to set the selected bit
-                 ;; If reg is 6, we need to clear the selected bit
-                 (x86
-                   (let* ((x86 (!flgi :cf
-                                      (the (unsigned-byte 1)
-                                           (acl2::logbit bitOffset bitBase))
-                                      x86))
-                          (x86 (!flgi-undefined :pf x86))
-                          (x86 (!flgi-undefined :af x86))
-                          (x86 (!flgi-undefined :sf x86))
-                          (x86 (!flgi-undefined :of x86)))
-                     x86))
-                 ((mv flg x86) (if (member reg '(5 6))  ;; If BTR, we need to clear the tested bit
-                                 (x86-operand-to-reg/mem
-                                   proc-mode
-                                   operand-size
-                                   inst-ac?
-                                   nil
-                                   (if (equal reg 5)
-                                     (logior bitBase
-                                             (ash 1 bitOffset))
-                                     (logand bitBase
-                                             (lognot (ash 1 bitOffset))))
-                                   seg-reg
-                                   addr
-                                   rex-byte
-                                   r/m
-                                   mod
-                                   x86)
-                                 (mv nil x86)))
-                 ((when flg) (!!ms-fresh :x86-operand-to-reg/mem flg))
-                 (x86 (write-*ip proc-mode temp-rip x86)))
-                x86)))
+                                 x86)
+                               (mv nil x86)))
+               ((when flg) (!!ms-fresh :x86-operand-to-reg/mem flg))
+               (x86 (write-*ip proc-mode temp-rip x86)))
+              x86)))
 
 ;; Helper for the bsr instruction
-(skip-proofs (defun bsr (source n)
-              (declare (xargs :verify-guards t))
-              (b* ((source>>1 (ash source -1))
-                   ((when (equal source>>1 0)) n))
-                  (bsr source>>1 (1+ n)))))
+(define bsr ((source integerp)
+             (n (and (integerp n)
+                     (<= 1 n))))
+  :guard (not (equal (loghead n source) 0))
+  :returns (bsr-result natp :hyp (and (integerp source)
+                                      (not (equal (loghead n source) 0))
+                                      (integerp n)
+                                      (<= 1 n))
+                       :hints (("Goal" :in-theory (enable natp))))
 
-(skip-proofs
-  (def-inst x86-bsr
-            ;; 0F BD/r: BSR r16. r/m16
-            ;; 0F BD/r: BSR r32. r/m32
-            ;; 0F BD/r: BSR r64. r/m64
+  :hints (("Goal" :in-theory (enable natp)))
+  :guard-debug t
 
-            ;; Note some odd behavior: According to Intel's manual,
-            ;; if the source operand is 0, the destination operand is undefined.
-            ;; AMD on the other hand states that it will be unchanged. I use the
-            ;; latter behavior. See also the comment at the end of BSF.
+  (if (mbt (and (integerp source)
+                (not (equal (loghead n source) 0))
+                (integerp n)
+                (<= 1 n)))
+    (b* (((when (equal (loghead (1- n) source) 0)) (1- n)))
+        (bsr source (1- n)))
+    nil)
+  ///
+  (defthm bsr-bound
+          (implies (and (integerp source)
+                        (not (equal (loghead n source) 0))
+                        (integerp n)
+                        (<= 1 n))
+                   (< (bsr source n)
+                      n))))
 
-            :parents (two-byte-opcodes)
 
-            :returns (x86 x86p :hyp (x86p x86))
+(skip-proofs (def-inst x86-bsr
+                       ;; 0F BD/r: BSR r16. r/m16
+                       ;; 0F BD/r: BSR r32. r/m32
+                       ;; 0F BD/r: BSR r64. r/m64
 
-            :guard-hints (("Goal" :in-theory (enable rme-size-of-1-to-rme08)))
+                       ;; Note some odd behavior: According to Intel's manual,
+                       ;; if the source operand is 0, the destination operand is undefined.
+                       ;; AMD on the other hand states that it will be unchanged. I use the
+                       ;; latter behavior. See also the comment at the end of BSF.
 
-            :modr/m t
+                       :parents (two-byte-opcodes)
 
-            :body
+                       :returns (x86 x86p :hyp (x86p x86))
 
-            ;; Note: opcode is the second byte of the two-byte opcode.
+                       :modr/m t
 
-            (b* (((the (integer 1 8) operand-size)
-                  (select-operand-size
-                    proc-mode nil rex-byte nil prefixes nil nil nil x86))
+                       :guard-hints (("Goal" :in-theory (e/d (natp) (unsigned-byte-p))))
 
-                 (p2 (prefixes->seg prefixes))
-                 (p4? (equal #.*addr-size-override*
-                             (prefixes->adr prefixes)))
+                       :prepwork
+                       ((local (defthm integerp-natp
+                                       (implies (natp x)
+                                                (integerp x)))))
 
-                 (seg-reg (select-segment-register proc-mode p2 p4? mod r/m sib x86))
+                       :body
 
-                 (inst-ac? t)
-                 ((mv flg0
-                      source
-                      (the (unsigned-byte 3) increment-RIP-by)
-                      (the (signed-byte 64) addr)
-                      x86)
-                  (x86-operand-from-modr/m-and-sib-bytes
-                    proc-mode #.*gpr-access* operand-size inst-ac?
-                    nil ;; Not a memory pointer operand
-                    seg-reg p4? temp-rip rex-byte r/m mod sib
-                    0 ;; No immediate data
-                    x86))
-                 ((when flg0)
-                  (!!ms-fresh :x86-operand-from-modr/m-and-sib-bytes flg0))
+                       ;; Note: opcode is the second byte of the two-byte opcode.
 
-                 ((mv flg (the (signed-byte #.*max-linear-address-size*) temp-rip))
-                  (add-to-*ip proc-mode temp-rip increment-RIP-by x86))
-                 ((when flg) (!!ms-fresh :rip-increment-error temp-rip))
+                       (b* (((the (integer 1 8) operand-size)
+                             (select-operand-size
+                               proc-mode nil rex-byte nil prefixes nil nil nil x86))
 
-                 (badlength? (check-instruction-length start-rip temp-rip 0))
-                 ((when badlength?)
-                  (!!fault-fresh :gp 0 :instruction-length badlength?)) ;; #GP(0)
+                            (p2 (prefixes->seg prefixes))
+                            (p4? (equal #.*addr-size-override*
+                                        (prefixes->adr prefixes)))
 
-                 ;; Update the x86 state:
-                 ;; ZF affected. CF, PF, AF, SF, and OF undefined.
-                 (x86 (if (equal source 0)
-                        x86
-                        (!rgfi-size operand-size (reg-index reg rex-byte *r*)
-                                    (bsr source 0) rex-byte x86)))
-                 (x86
-                   (let* ((x86 (!flgi :zf (if (equal source 0) 1 0) x86))
-                          (x86 (!flgi-undefined :cf x86))
-                          (x86 (!flgi-undefined :pf x86))
-                          (x86 (!flgi-undefined :af x86))
-                          (x86 (!flgi-undefined :sf x86))
-                          (x86 (!flgi-undefined :of x86)))
-                     x86))
-                 (x86 (write-*ip proc-mode temp-rip x86)))
-                x86)))
+                            (seg-reg (select-segment-register proc-mode p2 p4? mod r/m sib x86))
+
+                            (inst-ac? t)
+                            ((mv flg0
+                                 source
+                                 (the (unsigned-byte 3) increment-RIP-by)
+                                 (the (signed-byte 64) addr)
+                                 x86)
+                             (x86-operand-from-modr/m-and-sib-bytes
+                               proc-mode #.*gpr-access* operand-size inst-ac?
+                               nil ;; Not a memory pointer operand
+                               seg-reg p4? temp-rip rex-byte r/m mod sib
+                               0 ;; No immediate data
+                               x86))
+                            ((when flg0)
+                             (!!ms-fresh :x86-operand-from-modr/m-and-sib-bytes flg0))
+
+                            ((mv flg (the (signed-byte #.*max-linear-address-size*) temp-rip))
+                             (add-to-*ip proc-mode temp-rip increment-RIP-by x86))
+                            ((when flg) (!!ms-fresh :rip-increment-error temp-rip))
+
+                            (badlength? (check-instruction-length start-rip temp-rip 0))
+                            ((when badlength?)
+                             (!!fault-fresh :gp 0 :instruction-length badlength?)) ;; #GP(0)
+
+                            ;; Update the x86 state:
+                            ;; ZF affected. CF, PF, AF, SF, and OF undefined.
+                            (x86 (if (equal source 0)
+                                   x86
+                                   (!rgfi-size operand-size (reg-index reg rex-byte *r*)
+                                               (bsr source 64) rex-byte x86)))
+                            (x86
+                              (let* ((x86 (!flgi :zf (if (equal source 0) 1 0) x86))
+                                     (x86 (!flgi-undefined :cf x86))
+                                     (x86 (!flgi-undefined :pf x86))
+                                     (x86 (!flgi-undefined :af x86))
+                                     (x86 (!flgi-undefined :sf x86))
+                                     (x86 (!flgi-undefined :of x86)))
+                                x86))
+                            (x86 (write-*ip proc-mode temp-rip x86)))
+                           x86)))
 
 ;; Helper for the tzcnt instruction
-(skip-proofs (defun tzcnt (bits i n)
-               (declare (xargs :verify-guards t))
-               (b* (((when (equal bits i)) bits)
-                    ((unless (equal (logand n (ash 1 i)) 0)) i))
-                   (tzcnt bits (1+ i) n))))
+(define tzcnt ((bits natp)
+               (i natp)
+               (n natp))
+  :guard (<= i bits)
+  :returns (tzcnt-result :hyp (and (natp i)
+                                   (natp bits)
+                                   (<= i bits))
+                         (and (natp tzcnt-result)
+                              (<= tzcnt-result bits))
+                         :hints (("Goal" :in-theory (enable natp))))
+  :measure (acl2-count (- bits i))
+  :hints (("Goal" :in-theory (enable natp)))
+  (if (mbt (and (natp i)
+                (natp bits)
+                (<= i bits)))
+    (b* (((when (equal bits i)) bits)
+        ((when (logbitp i n)) i))
+       (tzcnt bits (1+ i) n))
+    nil))
 
-(skip-proofs
-  (def-inst x86-tzcnt
-            ;; F3 0F BC/r: TZCNT r16. r/m16
-            ;; F3 0F BC/r: TZCNT r32. r/m32
-            ;; F3 REX.W 0F BC/r: TZCNT r64. r/m64
+(skip-proofs (def-inst x86-tzcnt
+                       ;; F3 0F BC/r: TZCNT r16. r/m16
+                       ;; F3 0F BC/r: TZCNT r32. r/m32
+                       ;; F3 REX.W 0F BC/r: TZCNT r64. r/m64
 
-            :parents (two-byte-opcodes)
+                       :parents (two-byte-opcodes)
 
-            :returns (x86 x86p :hyp (x86p x86))
+                       :returns (x86 x86p :hyp (x86p x86))
 
-            :guard-hints (("Goal" :in-theory (enable rme-size-of-1-to-rme08)))
+                       :guard-hints (("Goal" :in-theory (e/d () ())))
 
-            :modr/m t
+                       :modr/m t
 
-            :body
+                       :body
 
-            ;; Note: opcode is the second byte of the two-byte opcode.
+                       ;; Note: opcode is the second byte of the two-byte opcode.
 
-            (b* (((the (integer 1 8) operand-size)
-                  (select-operand-size
-                    proc-mode nil rex-byte nil prefixes nil nil nil x86))
+                       (b* (((the (integer 1 8) operand-size)
+                             (select-operand-size
+                               proc-mode nil rex-byte nil prefixes nil nil nil x86))
 
-                 (p2 (prefixes->seg prefixes))
-                 (p4? (equal #.*addr-size-override*
-                             (prefixes->adr prefixes)))
+                            (p2 (prefixes->seg prefixes))
+                            (p4? (equal #.*addr-size-override*
+                                        (prefixes->adr prefixes)))
 
-                 (seg-reg (select-segment-register proc-mode p2 p4? mod r/m sib x86))
+                            (seg-reg (select-segment-register proc-mode p2 p4? mod r/m sib x86))
 
-                 (inst-ac? t)
-                 ((mv flg0
-                      source
-                      (the (unsigned-byte 3) increment-RIP-by)
-                      (the (signed-byte 64) addr)
-                      x86)
-                  (x86-operand-from-modr/m-and-sib-bytes
-                    proc-mode #.*gpr-access* operand-size inst-ac?
-                    nil ;; Not a memory pointer operand
-                    seg-reg p4? temp-rip rex-byte r/m mod sib
-                    0 ;; No immediate data
-                    x86))
-                 ((when flg0)
-                  (!!ms-fresh :x86-operand-from-modr/m-and-sib-bytes flg0))
+                            (inst-ac? t)
+                            ((mv flg0
+                                 source
+                                 (the (unsigned-byte 3) increment-RIP-by)
+                                 (the (signed-byte 64) addr)
+                                 x86)
+                             (x86-operand-from-modr/m-and-sib-bytes
+                               proc-mode #.*gpr-access* operand-size inst-ac?
+                               nil ;; Not a memory pointer operand
+                               seg-reg p4? temp-rip rex-byte r/m mod sib
+                               0 ;; No immediate data
+                               x86))
+                            ((when flg0)
+                             (!!ms-fresh :x86-operand-from-modr/m-and-sib-bytes flg0))
 
-                 ((mv flg (the (signed-byte #.*max-linear-address-size*) temp-rip))
-                  (add-to-*ip proc-mode temp-rip increment-RIP-by x86))
-                 ((when flg) (!!ms-fresh :rip-increment-error temp-rip))
+                            ((mv flg (the (signed-byte #.*max-linear-address-size*) temp-rip))
+                             (add-to-*ip proc-mode temp-rip increment-RIP-by x86))
+                            ((when flg) (!!ms-fresh :rip-increment-error temp-rip))
 
-                 (badlength? (check-instruction-length start-rip temp-rip 0))
-                 ((when badlength?)
-                  (!!fault-fresh :gp 0 :instruction-length badlength?)) ;; #GP(0)
+                            (badlength? (check-instruction-length start-rip temp-rip 0))
+                            ((when badlength?)
+                             (!!fault-fresh :gp 0 :instruction-length badlength?)) ;; #GP(0)
 
-                 (result (tzcnt (ash operand-size 3) 0 source))
+                            (result (tzcnt (ash operand-size 3) 0 source))
 
-                 ;; Update the x86 state:
-                 ;; ZF affected. CF, PF, AF, SF, and OF undefined.
-                 (x86 (!rgfi-size operand-size (reg-index reg rex-byte *r*)
-                                               result rex-byte x86))
-                 (x86
-                   (let* ((x86 (!flgi :zf (if (equal result 0) 1 0) x86))
-                          (x86 (!flgi :cf (if (equal source 0) 1 0) x86))
-                          (x86 (!flgi-undefined :pf x86))
-                          (x86 (!flgi-undefined :af x86))
-                          (x86 (!flgi-undefined :sf x86))
-                          (x86 (!flgi-undefined :of x86)))
-                     x86))
-                 (x86 (write-*ip proc-mode temp-rip x86)))
-                x86)))
+                            ;; Update the x86 state:
+                            ;; ZF affected. CF, PF, AF, SF, and OF undefined.
+                            (x86 (!rgfi-size operand-size (reg-index reg rex-byte *r*)
+                                             result rex-byte x86))
+                            (x86
+                              (let* ((x86 (!flgi :zf (if (equal result 0) 1 0) x86))
+                                     (x86 (!flgi :cf (if (equal source 0) 1 0) x86))
+                                     (x86 (!flgi-undefined :pf x86))
+                                     (x86 (!flgi-undefined :af x86))
+                                     (x86 (!flgi-undefined :sf x86))
+                                     (x86 (!flgi-undefined :of x86)))
+                                x86))
+                            (x86 (write-*ip proc-mode temp-rip x86)))
+                           x86)))
 
 ;; ======================================================================
