books/projects/x86isa/machine/instructions/cpuid.lisp
@@ -17,7 +17,10 @@
 ;; so I write my own set of cpuid info here
 
 (defaggregate cpuid-info
-              (eax ebx ecx edx))
+              ((eax (unsigned-byte-p 32 eax))
+               (ebx (unsigned-byte-p 32 ebx))
+               (ecx (unsigned-byte-p 32 ecx))
+               (edx (unsigned-byte-p 32 edx))))
 
 (defconst *cpuid-basic-info* (list (make-cpuid-info
                                      ;; Model and version info 
@@ -37,50 +40,70 @@
                                                   ))))
 (defconst *cpuid-extended-info* nil)
 
+(define valid-cpuid-info-list-p (val)
+  :guard t
+  (or (not val)
+      (and (consp val)
+           (cpuid-info-p (car val))
+           (valid-cpuid-info-list-p (cdr val)))))
+
 ;; Determine the correct cpu info for the given index and info set
-(skip-proofs (defun get-cpu-info (idx relevant-info)
-               (declare (xargs :verify-guards t))
-               (b* (((when (not relevant-info)) nil)
-                    ((when (equal idx 1)) (car relevant-info))
-                    (cpu-info (get-cpu-info (1- idx) (cdr relevant-info)))
-                    ((when (not cpu-info)) (car relevant-info)))
-                   cpu-info)))
+(define get-cpu-info ((idx natp)
+                      (relevant-info valid-cpuid-info-list-p))
+  :guard (not (equal idx 0))
+  :guard-hints (("Goal" :in-theory (enable valid-cpuid-info-list-p)))
+  (if (mbt (and (natp idx)
+                (not (equal idx 0))))
+    (b* (((when (not relevant-info)) nil)
+         ((when (equal idx 1)) (car relevant-info))
+         (cpu-info (get-cpu-info (1- idx) (cdr relevant-info)))
+         ((when (not cpu-info)) (car relevant-info)))
+        cpu-info)
+    nil)
+  ///
+  (defthm cpuid-info-p-get-cpu-info-nonnil
+          (implies (and (valid-cpuid-info-list-p info-list)
+                        info-list
+                        (natp idx)
+                        (not (equal idx 0)))
+                   (cpuid-info-p (get-cpu-info idx info-list)))
+          :hints (("Goal" :in-theory (enable valid-cpuid-info-list-p)))))
 
-(skip-proofs (def-inst x86-cpuid
+(def-inst x86-cpuid
 
-           ;; Op/En: ZO
-           ;; 0f A2
+          ;; Op/En: ZO
+          ;; 0f A2
 
-           :parents (two-byte-opcodes)
+          :parents (two-byte-opcodes)
 
-           :guard-hints (("Goal" :in-theory (e/d (riml08 riml32) ())))
+          :guard-hints (("Goal" :in-theory (e/d (get-cpu-info valid-cpuid-info-list-p) ())))
 
-           :returns (x86 x86p :hyp (x86p x86))
+          :returns (x86 x86p :hyp (x86p x86))
 
-           :body
+          :body
 
-           (b* ((requested-info (rr32 *eax* x86))
-                ;; Choose between basic and extended data
-                (basic-info? (< requested-info #x80000000))
-                (relevant-info (if basic-info?
-                                   *cpuid-basic-info*
-                                   *cpuid-extended-info*))
-                ;; This essentially removes the information about whether to use basic or extended data
-                ;; and lets us use this value to index into the separate lists
-                (info-idx (mod requested-info #x80000000))
-                (info (if (or (not relevant-info)
-                              (equal info-idx 0)) 
-                          ;; Handle the case when the index is 0 separately
-                          (make-cpuid-info :eax (+ (len relevant-info)
-                                                   (if basic-info?
-                                                       0
-                                                       #x80000000))
-                                           :ebx 0
-                                           :ecx 0
-                                           :edx 0)
-                          (get-cpu-info info-idx relevant-info)))
-                (x86 (wr32 *eax* (cpuid-info->eax info) x86))
-                (x86 (wr32 *ebx* (cpuid-info->ebx info) x86))
-                (x86 (wr32 *ecx* (cpuid-info->ecx info) x86))
-                (x86 (wr32 *edx* (cpuid-info->edx info) x86)))
-               (write-*ip proc-mode temp-rip x86))))
+          (b* ((requested-info (rr32 *eax* x86))
+               ;; Choose between basic and extended data
+               (basic-info? (< requested-info #x80000000))
+               (relevant-info (if basic-info?
+                                *cpuid-basic-info*
+                                *cpuid-extended-info*))
+               ;; This essentially removes the information about whether to use basic or extended data
+               ;; and lets us use this value to index into the separate lists
+               (info-idx (loghead 31 requested-info))
+               (info (if (or (not relevant-info)
+                             (equal info-idx 0)) 
+                       ;; Handle the case when the index is 0 separately
+                       (make-cpuid-info :eax (+ (len relevant-info)
+                                                (if basic-info?
+                                                  0
+                                                  #x80000000))
+                                        :ebx 0
+                                        :ecx 0
+                                        :edx 0)
+                       (get-cpu-info info-idx relevant-info)))
+               (x86 (wr32 *eax* (cpuid-info->eax info) x86))
+               (x86 (wr32 *ebx* (cpuid-info->ebx info) x86))
+               (x86 (wr32 *ecx* (cpuid-info->ecx info) x86))
+               (x86 (wr32 *edx* (cpuid-info->edx info) x86)))
+              (write-*ip proc-mode temp-rip x86)))
